\documentclass{article}
\usepackage{graphicx} % Required for inserting images
\usepackage[margin=1in]{geometry}
\usepackage[numbers]{natbib}
\usepackage{amsmath}
\bibliographystyle{plainnat}

\title{Basic Mathematics \cite{lang}}
\author{Garrett Moore}
\date{November 2023}

\renewcommand{\bibsection}{}

\begin{document}

\maketitle

\newpage
\section*{Chapter 1: Numbers}
\subsection*{Section 1.1: The Integers}

\newpage
\subsection*{Section 1.2: Rules for Addition}
\subsubsection*{Practice}
Justify each step, using commutativity and associativity in proving the following identities.\\
1. $(a + b) + (c + d) = (a + d) + (b + c)$\\
Answer:\\
\begin{align*}
    (a+b)+(c+d) &= a + b + c + d \hspace{3cm}\text{by associativity}\\
    &= a + d + b + c \hspace{3cm} \text{by commutativity}\\
    &= (a + d) + (b + c) \hspace{3cm} \text{by associativity}\\
\end{align*}

\noindent 3. $(a - b) + (c - d) = (a + c) + (-b - d)$\\
Answer:\\
\begin{align*}
    (a - b) + (c - d) &= a - b + c - d \hspace{3cm}\text{by associativity}\\
    &= a + c - b - d \hspace{3cm} \text{by commutativity}\\
    &= (a + c) + (-b - d) \hspace{3cm} \text{by associativity}\\
\end{align*}

\noindent 5. $(a - b) + (c - d) = (a - d) + (c - b)$\\
Answer:\\
\begin{align*}
    (a - b) + (c - d) &= a - b + c - d \hspace{3cm} \text{by associativity}\\
    &= a - d + c - b \hspace{3cm} \text{by commutativity}\\
    &= (a - d) + (c - b) \hspace{3cm} \text{by associativity}\\
\end{align*}

\noindent 7. $(a - b) + (c - d) = -(b + d) - (-a - c)$\\
Answer:\\
\begin{align*}
    (a - b) + (c - d) &= a - b + c - d \hspace{3cm} \text{by associativity}\\
    &= -b - d + a + c \hspace{3cm} \text{by commutativity}\\
    &= -(b + d) - (-a - c)
\end{align*}



\newpage
\section*{References}
\bibliography{bibfile}
    

\end{document}
